proof T_11_3_1_1

full-simpl/chap11.v
@@ -7,11 +7,11 @@ From Coq Require Import Lists.List.
 Extract Inductive list => "list" [ "[]" "(::)" ].
 Extraction Language OCaml.
 Import ListNotations.
-Load "../std".
 
 Module deBruijin.
 
 Module E11_1.
+Require Import Nat.
 
 Inductive ty : Type :=
 | Bool
@@ -80,26 +80,26 @@ Fixpoint getbinding (n : nat) (ctx: context) :=
     end
   end.
 
-Fixpoint shift (d k : nat) (t : term) : term :=
+Fixpoint shift (d : nat) (t : term) : term :=
 match t with
-| var x => var (if leb d x then x + k else x)
-| abs x T t' => abs x T (shift (S d) k t')
-| app t1 t2 => app (shift d k t1) (shift d k t2)
+| var x => var (if leb d x then (S x) else x)
+| abs x T t' => abs x T (shift (S d) t')
+| app t1 t2 => app (shift d t1) (shift d t2)
 | tru => tru
 | fls => fls
 | If t1 t2 t3 =>
-  If (shift d k t1) (shift d k t2) (shift d k t3)
+  If (shift d t1) (shift d t2) (shift d t3)
 | unit => unit
 | seq t1 t2 =>
-  seq (shift d k t1) (shift d k t2)
+  seq (shift d t1) (shift d t2)
 end.
 
 Fixpoint subst (d : nat) (s t: term) : term :=
 match t with
 | var x =>
-  if eqb_nat d x then s
+  if eqb d x then s
   else if ltb d x then var (pred x) else var x
-| abs x T t' => abs x T (subst (S d) (shift 0 1 s) t')
+| abs x T t' => abs x T (subst (S d) (shift 0 s) t')
 | app t1 t2 => app (subst d s t1) (subst d s t2)
 | tru => tru
 | fls => fls
@@ -163,132 +163,309 @@ Lemma leb_S_l : forall m n,
   leb (n + S m) n = false.
 Proof.
   induction n; simpl; intros; auto.
-  destruct eqb_nat eqn:IH1. apply eqb_eq in IH1. rewrite IH1 in IHn. rewrite leb_refl in IHn; inversion IHn.
-  apply leb_F in IHn. apply Nat.nle_gt in IHn. apply Nat.lt_lt_succ_r in IHn. apply lt_not_le in IHn.
-  apply leb_F in IHn. rewrite IHn; reflexivity.
 Qed.
 
-Lemma shift_sub : forall t1 t2 n m,
-    subst n t2 (shift n (S m) t1) = shift n m t1.
+Require Import PeanoNat.
+
+Lemma sub_shift : forall t1 t2 n,
+    subst n t2 (shift n t1) = t1.
 Proof.
   induction t1; intros; simpl; auto.
-  destruct leb eqn:IH1; destruct eqb_nat eqn:IH2; try apply eqb_eq in IH2; subst.
-  rewrite leb_S_l in IH1. inversion IH1.
-  apply le_leb in IH1. eapply le_plus_trans with (p:= (S m)) in IH1. apply leb_le in IH1. apply leb_neq_lt in IH1; auto. rewrite IH1. rewrite Nat.add_succ_r. simpl. reflexivity.
-  rewrite leb_refl in IH1; inversion IH1.
-  destruct ltb eqn:IH3. apply ltb_to_leb in IH3. rewrite IH3 in IH1; inversion IH1.
-  reflexivity.
-  rewrite IHt1. reflexivity.
-  rewrite IHt1_1, IHt1_2; reflexivity.
-  rewrite IHt1_1, IHt1_2, IHt1_3; reflexivity.
-  rewrite IHt1_1, IHt1_2; reflexivity.
-Qed.
-
-Lemma shift_0_t : forall t n,
-    shift n 0 t = t.
-Proof.
-  induction t; simpl; intros; auto.
-  rewrite <- plus_n_O. destruct leb; reflexivity.
-  rewrite IHt; reflexivity.
-  rewrite IHt1, IHt2; reflexivity.
-  rewrite IHt1, IHt2, IHt3; reflexivity.
-  rewrite IHt1, IHt2; reflexivity.
-Qed.
-
-Lemma shift_sub_1 : forall t1 t2 n,
-    subst n t2 (shift n 1 t1) = t1.
-Proof.
-  intros. rewrite shift_sub. rewrite shift_0_t. reflexivity.
-Qed.
-
-Fixpoint e t :=
-  match t with
-  | var x => var x
-  | abs x T t' => abs x T (e t')
-  | app t1 t2 => app (e t1) (e t2)
-  | If t1 t2 t3 => If (e t1) (e t2) (e t3)
-  | seq t1 t2 => app (abs "x" Unit (shift 0 1 (e t2))) (e t1)
-  | _ => t
-  end.
-
-Lemma shift_shift : forall t n d1 d2,
-    shift n d1 (shift n d2 t) = shift n (d2 + d1) t.
-Proof.
-  induction t; simpl; intros; auto.
   -
-    destruct (leb n0 n) eqn:IH1.
-    apply le_leb in IH1. eapply le_plus_trans with (p:= d2) in IH1.
-    apply leb_le in IH1. rewrite IH1. rewrite Nat.add_assoc. reflexivity.
-    rewrite IH1. reflexivity.
+    destruct leb eqn:IH1; destruct eqb eqn:IH2; try apply Nat.eqb_eq in IH2; subst.
+    apply Nat.leb_le in IH1. apply Nat.nle_succ_diag_l in IH1. inversion IH1.
+    apply Nat.leb_le in IH1. apply Lt.le_lt_n_Sm in IH1. apply Nat.ltb_lt in IH1. rewrite IH1. simpl. reflexivity.
+    rewrite Nat.leb_refl in IH1. inversion IH1.
+    assert (n0 <? n = false).
+    apply Nat.ltb_ge, Nat.lt_le_incl, Nat.leb_gt. apply IH1.
+    rewrite H. reflexivity.
   -
-    rewrite IHt. reflexivity.
+    rewrite IHt1. reflexivity.
   -
-    rewrite IHt1, IHt2. reflexivity.
+    rewrite IHt1_1, IHt1_2; reflexivity.
   -
-    rewrite IHt1, IHt2, IHt3; reflexivity.
+    rewrite IHt1_1, IHt1_2, IHt1_3; reflexivity.
   -
-    rewrite IHt1, IHt2; reflexivity.
+    rewrite IHt1_2, IHt1_1; reflexivity.
 Qed.
-
-Lemma leb_S_n_S : forall n m,
-    leb n m = leb (S n) (S m).
-Proof.
-  intros. destruct leb eqn:IH.
-  apply le_leb in IH. apply le_n_S in IH. apply leb_le in IH.
-  rewrite IH. reflexivity.
-  apply leb_F in IH. apply Nat.nle_gt in IH. apply lt_n_S in IH.
-  apply Nat.nle_gt in IH. apply leb_F in IH. rewrite IH; reflexivity.
-Qed.
-
 
 Notation "t1 ';' t2" := (seq t1 t2) (at level 50).
-Notation "'[' n ':=' t2 ']' t1" := (subst n t2 t1) (at level 100).
 
-Fixpoint e2t n t :=
+Fixpoint e2t t :=
   match t with
   | var x => var x
-  | abs x T t' => abs x T (e2t (S n) t')
-  | app t1 t2 => app (e2t n t1) (e2t n t2)
-  | If t1 t2 t3 => If (e2t n t1) (e2t n t2) (e2t n t3)
-  | seq t1 t2 => app (abs "x" Unit (shift n 1 (e2t n t2))) (e2t n t1)
+  | abs x T t' => abs x T (e2t t')
+  | app t1 t2 => app (e2t t1) (e2t t2)
+  | If t1 t2 t3 => If (e2t t1) (e2t t2) (e2t t3)
+  | t1; t2 => app (abs "x" Unit (shift 0 (e2t t2 ))) (e2t t1)
   | _ => t
   end.
 
-Lemma shift_e : forall t n1 n2,
-  e2t (S n1) (shift n2 1 t) = shift n2 1 (e2t n1 t) .
+Lemma shift_shift : forall t1 i k,
+    i < (S k) ->
+    shift (S k) (shift i t1 ) = shift i (shift k t1).
 Proof.
-  induction t; simpl; intros; auto.
-  rewrite IHt. reflexivity.
-  rewrite IHt1, IHt2; reflexivity.
-  rewrite IHt1, IHt2, IHt3; reflexivity.
-  rewrite IHt1, IHt2.
-Admitted.
+  induction t1; simpl; intros; auto.
+  -
+    destruct leb eqn:IH1; destruct (leb k n) eqn:IH2.
+    apply Nat.leb_le in IH1. apply le_S in IH1. apply Nat.leb_le in IH1. rewrite IH1. reflexivity.
+    rewrite IH1. reflexivity.
+
+    destruct n. apply Nat.leb_le in IH2. inversion IH2; subst. compute in H. apply le_S_n in H.
+    inversion H; subst. simpl in IH1. inversion IH1.
+
+    compute in H. apply le_S_n in H. apply Nat.leb_le in IH2. apply Nat.le_trans with (p:= (S n)) in H; auto.
+    apply Nat.leb_nle in IH1. apply IH1 in H. inversion H.
+    rewrite IH1.
+    destruct n; auto.
+    assert (k <=? n = false).
+    +
+      apply Nat.leb_nle. intro. apply le_S in H0. apply Nat.leb_nle in IH2. apply IH2. apply H0.
+    +
+    rewrite H0. reflexivity.
+  -
+    rewrite IHt1; auto. apply Lt.lt_n_S. apply H.
+  -
+    rewrite IHt1_1, IHt1_2; auto.
+  -
+    rewrite IHt1_1, IHt1_2, IHt1_3; auto.
+  -
+    rewrite IHt1_1, IHt1_2; auto.
+Qed.
+
+
+Notation "t1 '[[' n ':=' t2 ']]' " := (subst n t2 t1) (at level 20).
+Lemma shift_sub : forall t1 i j s,
+    j < (S i) ->
+    shift i (t1 [[ j := s]] ) = (shift (i + 1 ) t1) [[j := (shift i s) ]].
+Proof.
+  induction t1; simpl; intros; auto.
+  -
+    rewrite Nat.add_1_r.
+    destruct eqb eqn:IH1.
+    +
+      apply Nat.eqb_eq in IH1; subst.
+      apply Nat.nle_gt in H. apply Nat.leb_nle in H. rewrite H.
+      rewrite Nat.eqb_refl. reflexivity.
+    +
+      destruct ((S i) <=? n) eqn:IH2; simpl.
+      ++
+        apply Nat.leb_le in IH2. apply Nat.lt_le_trans with (p:= n) in H; auto. apply Nat.ltb_lt in H.
+        rewrite H; simpl.
+        destruct n. inversion H. simpl.
+        apply le_S_n in IH2. apply Nat.leb_le in IH2. rewrite IH2.
+        destruct (j =? (S(S n))) eqn:IH3. apply Nat.eqb_eq in IH3; subst.
+        apply Nat.ltb_lt in H. apply Nat.nlt_succ_diag_l in H. inversion H.
+        apply Nat.ltb_lt, Nat.lt_lt_succ_r, Nat.ltb_lt in H. rewrite H.
+        reflexivity.
+      ++
+        destruct (j <? n) eqn:IH3.
+        +++
+          rewrite IH1. simpl. destruct n; simpl. compute in H. apply le_S_n in H. destruct i; simpl; auto.
+          inversion H; subst. simpl in IH1. inversion IH1.
+          apply Nat.leb_nle, Nat.nle_gt, Lt.lt_S_n, Nat.nle_gt, Nat.leb_nle in IH2.
+          rewrite IH2. reflexivity.
+        +++
+          simpl. rewrite IH1.
+          apply Nat.leb_nle, Nat.nle_gt in IH2. compute in IH2.
+          apply le_S_n, Lt.le_lt_or_eq in IH2. destruct IH2.
+          apply Nat.nle_gt in H0. apply Nat.leb_nle in H0. rewrite H0; reflexivity.
+          subst. compute in H. apply le_S_n, Lt.le_lt_or_eq in H. destruct H.
+          apply Nat.ltb_lt in H. rewrite H in IH3. inversion IH3.
+          subst. rewrite Nat.eqb_refl in IH1. inversion IH1.
+  -
+    rewrite IHt1. rewrite shift_shift; auto.
+    apply Nat.lt_0_succ.
+    apply Lt.lt_n_S; auto.
+  -
+    rewrite IHt1_1, IHt1_2; auto.
+  -
+    rewrite IHt1_1, IHt1_2, IHt1_3; auto.
+  -
+    rewrite IHt1_1, IHt1_2; auto.
+Qed.
+
+Lemma shift_sub_lt : forall t1 s i j,
+    i < (S j) ->
+    shift i (t1 [[j := s]]) = (shift i t1) [[(S j) := shift i s]].
+Proof.
+ induction t1; simpl; intros; auto.
+   -
+    destruct eqb eqn:IH1.
+    +
+      apply Nat.eqb_eq in IH1; subst.
+      destruct leb eqn:IH2.
+      *
+        simpl. rewrite Nat.eqb_refl. reflexivity.
+      *
+        apply Nat.leb_nle in IH2. compute in H. apply le_S_n in H. induction IH2; auto.
+    +
+      destruct (j <? n) eqn:IH2.
+      *
+        destruct (i <=? n) eqn:IH3.
+        **
+          rewrite IH1. apply Nat.ltb_lt in IH2. apply Lt.lt_n_S in IH2. apply Nat.ltb_lt in IH2.
+          rewrite IH2. simpl. destruct n; try discriminate; simpl.
+          apply Nat.leb_le in IH3. apply Lt.le_lt_or_eq in IH3. destruct IH3; subst.
+          compute in H0. apply le_S_n in H0. apply Nat.leb_le in H0; rewrite H0. reflexivity.
+          apply Nat.ltb_lt in IH2. apply Lt.lt_S_n in IH2. apply Lt.lt_S_n in H.
+          apply Nat.nle_gt in IH2. compute in H. induction IH2. apply H.
+        **
+          destruct n; try discriminate; simpl.
+          apply Nat.leb_nle in IH3. apply Nat.nle_gt in IH3. apply Nat.lt_succ_l in IH3. apply Nat.nle_gt in IH3. apply Nat.leb_nle in IH3. rewrite IH3.
+          destruct (j =? n) eqn:IH4. apply Nat.eqb_eq in IH4; subst. compute in H. apply Nat.leb_nle in IH3. apply le_S_n in H. induction IH3; apply H.
+          destruct (S j <? S n) eqn:IH5; auto.
+          apply Nat.ltb_lt in IH2. compute in IH2. apply Lt.le_lt_or_eq in IH2. destruct IH2; subst; try discriminate.
+          apply Nat.ltb_lt in H0. rewrite H0 in IH5. inversion IH5. inversion H0; subst. rewrite Nat.eqb_refl in IH4. inversion IH4.
+      *
+        destruct leb eqn:IH3.
+        **
+          rewrite IH1. simpl. rewrite IH3. destruct (S j <? S n) eqn:IH4; auto.
+          apply Nat.ltb_lt, Lt.lt_S_n, Nat.ltb_lt in IH4. rewrite IH4 in IH2. inversion IH2.
+        **
+          destruct n; simpl. rewrite IH3. reflexivity.
+          rewrite IH3. destruct (j =? n) eqn:IH4.
+          apply Nat.eqb_eq in IH4; subst. apply Nat.ltb_nlt in IH2. apply Nat.nlt_ge in IH2. einduction Nat.nle_succ_diag_l. apply IH2.
+          destruct (S j <? S n) eqn:IH5; auto.
+          apply Nat.ltb_lt in IH5. compute in IH5. repeat apply Le.le_Sn_le in IH5.
+          apply Lt.le_lt_or_eq in IH5; destruct IH5; subst. apply Nat.ltb_lt in H0. rewrite H0 in IH2. inversion IH2.
+          rewrite Nat.eqb_refl in IH1. inversion IH1.
+  -
+    rewrite IHt1; auto. rewrite shift_shift; auto.
+    apply Nat.lt_0_succ.
+    apply Lt.lt_n_S; auto.
+  -
+    rewrite IHt1_1; try rewrite IHt1_2; auto.
+  -
+    rewrite IHt1_1, IHt1_2, IHt1_3; auto.
+  -
+    rewrite IHt1_1, IHt1_2; auto.
+Qed.
+
+Lemma subsub :forall t1 j i v u,
+    i < (S j) ->
+    t1[[ S j := shift i v ]] [[i := u[[j := v ]] ]] = t1 [[i := u ]] [[j := v]].
+Proof.
+  induction t1; simpl; intros; auto.
+  -
+    destruct n.
+    +
+      destruct ltb eqn:IH1. inversion IH1.
+      simpl. destruct i. reflexivity.
+      simpl. apply Lt.lt_S_n in H. destruct j. inversion H. simpl. reflexivity.
+    +
+      simpl.
+      destruct eqb eqn:IH1.
+      ++
+        apply Nat.eqb_eq in IH1; subst. generalize H; intros. compute in H. destruct eqb eqn:IH1; try apply Nat.eqb_eq in IH1; subst.
+        einduction Nat.nle_succ_diag_l; eauto. apply Nat.ltb_lt in H0. rewrite H0. simpl. rewrite Nat.eqb_refl.
+        rewrite sub_shift. reflexivity.
+      ++
+        destruct ltb eqn:IH2; simpl.
+        destruct (eqb i n) eqn:IH3. apply Nat.eqb_eq in IH3; subst.
+        apply Nat.ltb_lt in IH2.
+        apply Nat.nle_gt in IH2. compute in H. induction IH2. apply H.
+      --
+        destruct (ltb i n) eqn:IH4.
+        destruct (i =? S n) eqn:IH5; try apply Nat.eqb_eq in IH5; subst. apply Nat.ltb_lt in IH4.
+        induction (Nat.nlt_succ_diag_l n); apply IH4.
+        apply Nat.ltb_lt in IH2. apply Nat.lt_trans with (p:= S n) in H; auto. apply Nat.ltb_lt in H. rewrite H.
+        simpl. rewrite IH1. apply Lt.lt_S_n in IH2. apply Nat.ltb_lt in IH2. rewrite IH2. reflexivity.
+        destruct (i =? S n) eqn:IH5; try apply Nat.eqb_eq in IH5; subst.
+        apply Nat.ltb_lt in IH2. apply Nat.nle_gt in IH2. apply Nat.lt_le_incl in H. induction IH2. apply H.
+        apply Nat.ltb_lt in IH2. apply Nat.lt_trans with (p:= S n) in H; auto. compute in H.
+        apply le_S_n in H. apply Lt.le_lt_or_eq in H. destruct H.
+        apply Nat.ltb_lt in H. rewrite H in IH4. inversion IH4.
+        subst. rewrite Nat.eqb_refl in IH3. inversion IH3.
+      --
+        destruct (i =? S n) eqn:IH3; try apply Nat.eqb_eq in IH3; subst; auto.
+        apply Nat.ltb_nlt in IH2. apply Nat.nlt_ge in IH2.
+        destruct (i <? S n) eqn:IH4. simpl.
+        rewrite IH1. apply le_S_n in IH2. apply Nat.nlt_ge in IH2. apply Nat.ltb_nlt in IH2. rewrite IH2. reflexivity.
+        simpl.
+        destruct (eqb j (S n)) eqn:IH5; try apply Nat.eqb_eq in IH5; subst.
+        ***
+          compute in H. apply le_S_n in H. apply Lt.le_lt_or_eq in H. destruct H; subst.
+          apply Nat.ltb_nlt in IH4. induction IH4; apply H.
+          rewrite Nat.eqb_refl in IH3. inversion IH3.
+        ***
+          destruct (ltb j (S n)) eqn:IH6; auto.
+          apply Nat.ltb_lt in IH6. compute in IH6.
+          apply Nat.lt_le_trans with (p:= S n) in H; auto. apply Nat.ltb_lt in H. rewrite H in IH4.
+          inversion IH4.
+  -
+    generalize Nat.lt_0_succ; intros.
+    generalize H; intros.
+    apply Lt.lt_n_S in H. apply IHt1 with (v:= v) (u:= u) in H.
+    rewrite shift_sub_lt; auto. rewrite <- shift_shift; auto. rewrite IHt1. reflexivity. apply Lt.lt_n_S.
+    apply H1.
+  -
+    rewrite IHt1_2, IHt1_1; auto.
+  -
+    rewrite IHt1_1, IHt1_2, IHt1_3; auto.
+  -
+    rewrite IHt1_2, IHt1_1; auto.
+Qed.
+
+Lemma shift_e2t : forall t1 n,
+    e2t (shift n t1) = shift n (e2t t1).
+Proof.
+  induction t1; simpl; intros; auto.
+  -
+    rewrite IHt1; reflexivity.
+  -
+    rewrite IHt1_1, IHt1_2; reflexivity.
+  -
+    rewrite IHt1_1, IHt1_2, IHt1_3; reflexivity.
+  -
+    rewrite shift_shift; auto.
+    rewrite IHt1_1. rewrite IHt1_2. reflexivity.
+    compute. apply le_n_S. apply le_0_n.
+Qed.    
 
 Lemma subst_e2t : forall t1 t2 n,
-    e2t n ([n := t2]t1) = ([n := (e2t n t2)](e2t (S n) t1)).
+   e2t (t1[[n := t2]] ) = (e2t t1)[[n:= (e2t t2)]].
 Proof.
-  induction t1; simpl; intros; eauto.
-  destruct eqb_nat; eauto.
-  destruct ltb; auto.
-  rewrite IHt1.
-  rewrite shift_e. reflexivity.
-  rewrite IHt1_1, IHt1_2; reflexivity.
-  rewrite IHt1_1, IHt1_2, IHt1_3; reflexivity.
-  rewrite IHt1_1, IHt1_2.
-Admitted.
-
-Theorem T11_3_1_1_1__ : forall t t',
-  t -->e t' ->
-  (e2t 0 t) -->i (e2t 0 t').
-Proof.
-  induction t; intros; simpl; try solve_by_inverts 2.
+  induction t1; simpl; intros; auto.
   -
-    inversion H; subst; simpl; try constructor; auto.
+    destruct eqb; destruct ltb; auto.
+  -
+    rewrite IHt1, shift_e2t. reflexivity.
+  -
+    rewrite IHt1_1, IHt1_2; auto.
+  -
+    rewrite IHt1_1, IHt1_2, IHt1_3; reflexivity.
+  -
+    rewrite IHt1_1, IHt1_2.
+    rewrite shift_sub_lt. reflexivity.
+    compute. apply le_n_S. apply le_0_n.
+Qed.    
+
+Ltac solve_by_inverts n :=
+  match goal with | H : ?T |- _ =>
+  match type of T with Prop =>
+    solve [
+      inversion H;
+      match n with S (S (?n')) => subst; solve_by_inverts (S n') end ]
+  end end.
+
+Ltac solve_by_invert :=
+  solve_by_inverts 1.
+
+
+Theorem T11_3_1_1_1 : forall t' t'',
+  t' -->e t'' ->
+  (e2t t') -->i (e2t t'').
+Proof.
+  induction t'; intros; simpl; try solve_by_inverts 2.
+  -
+    inversion H; subst; simpl; try solve [constructor; auto].
     +
-      destruct t1; try solve_by_invert; constructor.
+      apply IHt'2 in H4. apply Ei_App2; auto. destruct t'1; simpl; try constructor; solve_by_invert; auto.
     +
-      rewrite subst_e2t; auto. constructor.
-      destruct t2; try solve_by_invert; constructor.
+      rewrite subst_e2t; auto.
+      constructor.
+      destruct t'2; try constructor; solve_by_invert.
   -
     inversion H; subst; simpl; try constructor; auto.
   -
@@ -296,45 +473,13 @@ Proof.
     +
       constructor.
     +
-      erewrite <- shift_sub_1.  constructor. destruct t1; try solve_by_invert; constructor.
-Qed.
+      erewrite <- sub_shift. constructor. destruct t'1; try solve_by_invert; constructor.
+Qed.    
 
-Lemma subst_e : forall t1 t2 n,
-    e (subst n t2 t1) = subst n (e t2) (e t1).
-Proof.
-  induction t1; intros; simpl; auto; try solve_by_invert.
-  destruct eqb_nat; auto.
-  destruct ltb; auto.
-  rewrite IHt1. admit.
-  rewrite IHt1_1, IHt1_2; reflexivity.
-  rewrite IHt1_1, IHt1_2, IHt1_3; reflexivity.
-  rewrite IHt1_1, IHt1_2.
-Admitted.
-
-Theorem T11_3_1_1_1 : forall t t',
-  t -->e t' ->
-  (e t) -->i (e t').
-Proof.
-  induction t; intros; simpl; try solve_by_inverts 2.
-  -
-    inversion H; subst; simpl; try constructor; auto.
-    +
-      destruct t1; try solve_by_invert; constructor.
-    +
-      rewrite subst_e; auto. constructor; destruct t2; try solve_by_invert; constructor.
-  -
-    inversion H; subst; simpl; try constructor; auto.
-  -
-    inversion H; subst; simpl; try constructor; auto; try solve_by_invert.
-    +
-      constructor.
-    +
-      erewrite <- shift_sub_1. constructor. destruct t1; try solve_by_invert; constructor.
-Qed.
 
 Theorem T11_3_1_1_2 : forall t u,
-  (e t) -->i u ->
-  exists t', u = e t' /\ t -->e t'.
+  (e2t t) -->i u ->
+  exists t', u = e2t t' /\ t -->e t'.
 Proof.
   induction t; simpl; intros; try solve_by_invert.
   -
@@ -346,7 +491,7 @@ Proof.
       destruct t1; try solve_by_invert; constructor.
     +
       destruct t1; try solve_by_invert. simpl in H0. inversion H0; subst.
-      exists (subst 0 t2 t1). split. symmetry. apply subst_e.
+      exists (subst 0 t2 t1). split. symmetry. apply subst_e2t.
       constructor.
       destruct t2; try solve_by_invert; constructor.
   -
@@ -365,7 +510,7 @@ Proof.
     +
       apply IHt1 in H4. destruct H4; destruct H0; subst. exists (seq x t2); split; try constructor; auto.
     +
-      exists t2. split; try constructor; auto. apply shift_sub_1. destruct t1; try solve_by_invert; constructor.
+      exists t2. split; try constructor; auto. apply sub_shift. destruct t1; try solve_by_invert; constructor.
 Qed.
 
 Reserved Notation "ctx '|-' t '\in' T" (at level 40).
@@ -403,7 +548,7 @@ Lemma appGetbind : forall ctx ctx' n,
 Proof.
   induction ctx; simpl; intros; auto.
   rewrite <- plus_n_O; reflexivity.
-  rewrite <- plus_Snm_nSm. simpl. apply IHctx.
+  rewrite Nat.add_succ_r. simpl. apply IHctx.
 Qed.
 
 Lemma length1_Some : forall n ctx ctx1 ctx2 T,
@@ -413,326 +558,26 @@ Lemma length1_Some : forall n ctx ctx1 ctx2 T,
 Proof.
   induction n; simpl; intros. destruct ctx. inversion H. simpl. simpl in H0. apply H0.
   destruct ctx. inversion H. simpl. destruct ( (p :: ctx) ++ ctx1) eqn:IHH. inversion H0. inversion IHH; subst.
-  eapply IHn in H0. apply H0. simpl in H. apply lt_S_n in H. apply H.
+  eapply IHn in H0. apply H0. simpl in H. apply Lt.lt_S_n in H. apply H.
 Qed.
 
-Lemma shifting : forall t g g1 g2 T,
-  (g1 ++ g) |- t \in T ->
-  (g1 ++ g2 ++ g) |- (shift (length g1) (length g2) t) \in T.
+Theorem T11_3_1_2 : forall t1 T ctx,
+    ctx |- t1 \in T <->
+    ctx |- (e2t t1) \in T.
 Proof.
-  induction t; intros; inversion H; subst; clear H; try solve [econstructor; eauto]; simpl.
-
-  apply T_Var. destruct (leb) eqn:IH. apply le_leb in IH.
-  generalize dependent g. generalize dependent T. generalize dependent n.
-  induction g1; simpl; intros; eauto. unfold getbinding. rewrite appGetbind. apply H2.
-  destruct n. inversion IH. simpl.
-  apply le_S_n in IH. simpl in H2. eapply IHg1 in IH; eauto.
-
-  apply leb_neq in IH. eapply length1_Some in IH. apply IH. apply H2.
-
-  apply T_Abs.
-  assert (S (length g1) = length ((name, typ) :: g1)). reflexivity.
-  rewrite H. apply IHt with (g1:= ((name, typ) :: g1)). apply H5.
-Qed.
-
-Lemma shifting_l : forall t g g1 g2 T,
-  (g1 ++ g2 ++ g) |- (shift (length g1) (length g2) t) \in T ->
-  (g1 ++ g) |- t \in T.
-Proof.
-  induction t; intros; inversion H; subst; clear H; try solve [econstructor; eauto]; simpl.
+  split; generalize dependent T; generalize dependent ctx.
   -
-    apply T_Var. destruct (leb) eqn:IH. apply le_leb in IH.
-    generalize dependent g. generalize dependent T. generalize dependent n.
-    induction g1; simpl; intros; eauto. unfold getbinding in H2. rewrite appGetbind in H2. apply H2.
-    destruct n. inversion IH. simpl.
-    apply le_S_n in IH. simpl in H2. eapply IHg1 in IH; eauto.
-    apply leb_neq in IH. eapply length1_Some in IH. apply IH. apply H2.
-  -
-    apply T_Abs.
-    assert (S (length g1) = length ((name, typ) :: g1)). reflexivity. rewrite H in H5.
-    eapply IHt with (g1:= ((name, typ) :: g1)). apply H5.
-Qed.
-
-Theorem T11_3_1_2 : forall t T ctx n,
-    ctx |- t \in T <->
-    ctx |- (e2t n t) \in T.
-Proof.
-  split; generalize dependent T; generalize dependent ctx; generalize dependent n.
-  -
-    induction t; simpl; intros; auto; inversion H; subst; try solve [econstructor; eauto].
+    induction t1; simpl; intros; auto; inversion H; subst; try solve [econstructor; eauto].
     +
       econstructor; eauto. constructor; auto.
       admit.
   -
-    induction t; simpl; intros; auto; inversion H; subst; try solve [econstructor; eauto].
+    induction t1; simpl; intros; auto; inversion H; subst; try solve [econstructor; eauto].
     inversion H3; subst.
-    constructor; eauto. eapply IHt2.
+    constructor; eauto.
     admit.
 Abort.
 
-(*
-Theorem T11_3_1_2 : forall t T ctx,
-    ctx |- t \in T <->
-    ctx |- (e2t t) \in T.
-Proof.
-  split; generalize dependent T; generalize dependent ctx.
-  -
-    induction t; simpl; intros; auto; inversion H; subst; try solve [econstructor; eauto].
-    +
-      econstructor. constructor; auto.
-      assert (("x"%string, Unit) :: ctx = [] ++ [("x"%string, Unit)] ++ ctx). reflexivity. rewrite H0.
-      apply shifting. simpl. apply IHt2. apply H5.
-      apply IHt1. apply H3.
-  -
-    induction t; simpl; intros; inversion H; subst; try solve [econstructor; eauto].
-    inversion H3; subst. apply T_Seq. apply IHt1. apply H5. apply IHt2.
-    assert (ctx = [] ++ ctx). reflexivity. rewrite H0.
-    eapply shifting_l with (g2:= [("x"%string, Unit)]).
-    assert ([] ++ [("x"%string, Unit)] ++ ctx = [("x"%string, Unit)] ++ ctx). reflexivity.
-    apply H2.
-Qed.
-*)
 End E11_1.
 
 End deBruijin.
-
-Module string.
-
-Module Seq.
-Inductive ty : Type :=
-| Bool
-| Unit
-|Arrow (ty1 ty2: ty) .
-Notation "t1 '|-->' t2" := (Arrow t1 t2) (at level 40).
-
-Inductive term : Type :=
-(*純粋λ計算*)
-| var (name: string)
-| abs (name: string) (typ: ty) (t: term)
-| app (t1 t2: term)
-(*ぶーる*)
-| tru
-| fls
-| unit
-| If (t1 t2 t3: term)
-| seq (t1 t2: term).
-
-Inductive value : term -> Prop :=
-  | v_abs : forall x T t, value (abs x T t)
-  | v_tru : value tru
-  | v_fls : value fls
-  | v_uni : value unit.
-
-Reserved Notation "'[' x ':=' s ']' t" (at level 20).
-
-Fixpoint subst (x : string) (s : term) (t : term) : term :=
-  match t with
-  | var x' => if String.eqb x x' then s else t
-  | abs x' T t1 => abs x' T (if String.eqb x x' then t1 else ([x:=s] t1))
-  | app t1 t2 => app ([x:=s] t1) ([x:=s] t2)
-  | tru => tru
-  | fls => fls
-  | unit => unit
-  | If t1 t2 t3 => If ([x:=s] t1) ([x:=s] t2) ([x:=s] t3)
-  | seq t1 t2 => seq ([x:=s]t1) ([x:=s]t2)
-  end
-
-where "'[' x ':=' s ']' t" := (subst x s t).
-
-Reserved Notation "t1 '-->' t2" (at level 40).
-
-Inductive step : term -> term -> Prop :=
-  | E_AppAbs : forall x T t12 v2,
-         value v2 ->
-         (app (abs x T t12) v2) --> [x:=v2]t12
-  | E_App1 : forall t1 t1' t2,
-         t1 --> t1' ->
-         app t1 t2 --> app t1' t2
-  | E_App2 : forall v1 t2 t2',
-         value v1 ->
-         t2 --> t2' ->
-         app v1 t2 --> app v1 t2'
-  | E_IfTru : forall t1 t2,
-      (If tru t1 t2) --> t1
-  | E_IfFls : forall t1 t2,
-      (If fls t1 t2) --> t2
-  | E_If : forall t1 t1' t2 t3,
-      t1 --> t1' ->
-      (If t1 t2 t3) --> (If t1' t2 t3)
-  | E_seq : forall t1 t1' t2,
-      t1 --> t1' ->
-      seq t1 t2 --> seq t1' t2
-  | E_SeqNext : forall v1 t2,
-      value v1 ->
-      seq v1 t2 --> t2
-
-where "t1 '-->' t2" := (step t1 t2).
-
-
-Definition context := partial_map ty.
-
-Inductive appears_free_in : string -> term -> Prop :=
-  | afi_var : forall x,
-      appears_free_in x (var x)
-  | afi_app1 : forall x t1 t2,
-      appears_free_in x t1 ->
-      appears_free_in x (app t1 t2)
-  | afi_app2 : forall x t1 t2,
-      appears_free_in x t2 ->
-      appears_free_in x (app t1 t2)
-  | afi_abs : forall x y T11 t12,
-      y <> x ->
-      appears_free_in x t12 ->
-      appears_free_in x (abs y T11 t12)
-  | afi_test1 : forall x t1 t2 t3,
-      appears_free_in x t1 ->
-      appears_free_in x (If t1 t2 t3)
-  | afi_test2 : forall x t1 t2 t3,
-      appears_free_in x t2 ->
-      appears_free_in x (If t1 t2 t3)
-  | afi_test3 : forall x t1 t2 t3,
-      appears_free_in x t3 ->
-      appears_free_in x (If t1 t2 t3)
-  | afi_seq1 : forall x t1 t2,
-      appears_free_in x t1 ->
-      appears_free_in x (seq t1 t2)
-  | afi_seq2 : forall x t1 t2,
-      appears_free_in x t2 ->
-      appears_free_in x (seq t1 t2).
-
-Notation "x '∈fv' t" := (appears_free_in x t) (at level 50).
-
-Fixpoint free x t :=
-  match t with
-  | var x' => eqb x x'
-  | app t1 t2 =>
-    orb (free x t1) (free x t2)
-  | abs y T t1 =>
-    if eqb x y then false
-    else free x t1
-  | If t1 t2 t3 =>
-    (free x t1) || (free x t2) || (free x t3)
-  | tru => false
-  | fls => false
-  | unit => false
-  | seq t1 t2 =>
-    (free x t1) || (free x t2)
-  end.
-
-Fixpoint e x t :=
-  match t with
-  | abs s T t' => abs s T (e x t')
-  | app t1 t2 => app (e x t1) (e x t2)
-  | If t1 t2 t3 => If (e x t1) (e x t2) (e x t3)
-  | seq t1 t2 => app (abs x Unit (e x t2)) (e x t1)
-  | _ => t
-  end.
-
-Open Scope string.
-Lemma subst_e_free : forall t1 t2 x,
-    not (x ∈fv t1) ->
-    [x := t2]t1 = t1.
-Proof.
-  induction t1; simpl; intros; auto;
-    try (rewrite IHt1_1, IHt1_2; try rewrite IHt1_3; auto; intro; apply H; solve [constructor; auto]).
-  -
-    destruct eqb eqn:IH; auto. apply String.eqb_eq in IH; subst.
-    induction H. constructor.
-  -
-    destruct eqb eqn:IH; auto. rewrite IHt1; auto.
-    intro. apply H. constructor. intro. subst. rewrite String.eqb_refl in IH.
-    inversion IH. apply H0.
-Qed.
-
-
-Lemma afi_e : forall t x,
-    x ∈fv e x t -> x ∈fv t.
-Proof.
-  induction t; simpl; intros; auto.
-  inversion H; subst. constructor; auto.
-  inversion H; subst; solve [constructor; auto].
-  inversion H; subst; solve [constructor; auto].
-  inversion H; subst; try solve [constructor; auto].
-  inversion H2; subst. solve [constructor; auto].
-Qed.
-
-
-Lemma subst_e : forall t1 t2 x x',
-    not (x' ∈fv t1) ->
-    e x ([x':= t2]t1) = [x' := e x t2](e x t1).
-Proof.
-  induction t1; simpl; intros; auto.
-  destruct eqb; auto.
-  destruct eqb eqn:IH. apply String.eqb_eq in IH; subst; auto.
-  rewrite IHt1; auto.
-  intro. apply H. constructor. intro; subst. rewrite String.eqb_refl in IH. inversion IH. apply H0.
-  rewrite IHt1_1, IHt1_2; auto; intro; apply H; solve [constructor; auto].
-  rewrite IHt1_1, IHt1_2, IHt1_3; auto; intro; apply H; solve [constructor; auto].
-  rewrite IHt1_1, IHt1_2; auto. destruct eqb eqn:IH; auto. apply String.eqb_eq in IH; subst.
-  rewrite subst_e_free. reflexivity.
-  intro. apply H. apply afi_seq2. apply afi_e. apply H0.
-  intro. apply H; solve [constructor; auto].
-  intro. apply H; solve [constructor; auto].
-Qed.
-
-Theorem T11_3_1_1 : forall t t' x,
-  t --> t' ->
-  not (x ∈fv t) -> not (x ∈fv t') ->
-  e x t --> e x t'.
-Proof.
-  induction t; simpl; intros; try solve_by_invert.
-  -
-    inversion H; subst.
-    +
-      rewrite subst_e. constructor; auto. destruct t2; try solve_by_invert; constructor.
-      admit.
-    +
-      constructor. apply IHt1; auto.
-      intro; apply H0; constructor; auto.
-      intro; apply H1; constructor; auto.
-    +
-      constructor; auto. destruct t1; try solve_by_invert; constructor.
-      apply IHt2; auto; intro.
-      apply H0; solve[constructor; auto].
-      apply H1; solve[constructor; auto].
-  -
-    inversion H; subst; simpl; try constructor; auto.
-    apply IHt1; auto; intro. apply H0; constructor; auto.
-    apply H1; solve[constructor; auto].
-  -
-    inversion H; subst; simpl.
-    +
-      constructor; auto. destruct t2; try solve_by_invert; constructor.
-      apply IHt1; auto; intro.
-      apply H0; constructor; auto.
-      apply H1; constructor; auto.
-Admitted.
-
-
-Reserved Notation "ctx '|-' t '\in' T" (at level 40).
-Inductive has_type : context -> term -> ty -> Prop :=
-  | T_Var : forall ctx x T,
-      ctx x = Some T ->
-      ctx |- var x \in T
-  | T_Abs : forall ctx x T11 T12 t12,
-      (x |-> T11 ; ctx) |- t12 \in T12 ->
-      ctx |- abs x T11 t12 \in Arrow T11 T12
-  | T_App : forall T11 T12 ctx t1 t2,
-      ctx |- t1 \in Arrow T11 T12 ->
-      ctx |- t2 \in T11 ->
-      ctx |- app t1 t2 \in T12
-  | T_Tru : forall ctx,
-       ctx |- tru \in Bool
-  | T_Fls : forall ctx,
-       ctx |- fls \in Bool
-  | T_If : forall t1 t2 t3 T ctx,
-       ctx |- t1 \in Bool ->
-       ctx |- t2 \in T ->
-       ctx |- t3 \in T ->
-       ctx |- If t1 t2 t3 \in T
-
-where "ctx '|-' t '\in' T" := (has_type ctx t T).
-
-End Seq.
-
-End string.
